{
  "@id": "https://stencila.org/CodeLocation",
  "name": "CodeLocation",
  "license": "https://creativecommons.org/publicdomain/zero/1.0/",
  "@context": {
    "rdfs": "http://www.w3.org/2000/01/rdf-schema#",
    "schema": "https://schema.org/",
    "stencila": "https://stencila.org/"
  },
  "@graph": [
    {
      "@id": "stencila:CodeLocation",
      "@type": "rdfs:Class",
      "rdfs:label": "CodeLocation",
      "rdfs:comment": "The location within some source code.",
      "rdfs:subClassOf": {
        "@id": "stencila:Entity"
      }
    },
    {
      "@id": "stencila:source",
      "@type": "rdfs:Property",
      "rdfs:label": "source",
      "rdfs:comment": "The source of the code, a file path, label or URL.",
      "schema:domainIncludes": [
        {
          "@id": "stencila:CodeLocation"
        },
        {
          "@id": "stencila:IncludeBlock"
        }
      ],
      "schema:rangeIncludes": {
        "@id": "schema:Text"
      }
    },
    {
      "@id": "stencila:startLine",
      "@type": "rdfs:Property",
      "rdfs:label": "startLine",
      "rdfs:comment": "The 1-based index if the first line on which the error occurred.",
      "schema:domainIncludes": {
        "@id": "stencila:CodeLocation"
      },
      "schema:rangeIncludes": {
        "@id": "stencila:UnsignedInteger"
      }
    },
    {
      "@id": "stencila:startColumn",
      "@type": "rdfs:Property",
      "rdfs:label": "startColumn",
      "rdfs:comment": "The 1-based index if the first column on which the error occurred.",
      "schema:domainIncludes": {
        "@id": "stencila:CodeLocation"
      },
      "schema:rangeIncludes": {
        "@id": "stencila:UnsignedInteger"
      }
    },
    {
      "@id": "stencila:endLine",
      "@type": "rdfs:Property",
      "rdfs:label": "endLine",
      "rdfs:comment": "The 1-based index if the last line on which the error occurred.",
      "schema:domainIncludes": {
        "@id": "stencila:CodeLocation"
      },
      "schema:rangeIncludes": {
        "@id": "stencila:UnsignedInteger"
      }
    },
    {
      "@id": "stencila:endColumn",
      "@type": "rdfs:Property",
      "rdfs:label": "endColumn",
      "rdfs:comment": "The 1-based index if the last column on which the error occurred.",
      "schema:domainIncludes": {
        "@id": "stencila:CodeLocation"
      },
      "schema:rangeIncludes": {
        "@id": "stencila:UnsignedInteger"
      }
    }
  ]
}